refinement proof for the timer driver (wo u32/volatile)

timer/TimerSpec.thy
@@ -1,477 +1,117 @@
 theory TimerSpec
-  imports Main "HOL-Word.Word" "Word_Lib.Word_Lib" 
+  imports Main
 begin
 
-record ('s, 'time, 'timeout) driver =
-  (*  invariants 
-   dataInv :: "'s \<Rightarrow> bool"
-   brightnessInv :: "'b \<Rightarrow> bool"
-   indexInv :: "'s \<Rightarrow> 'i \<Rightarrow> bool"    *)
-  (*  interface *)
-(* TODO: replace 'n with nat, or better, remove this field *)
+record ('s, 'reg, 'time, 'timeout, 'timer_mode) driver =
    get_time :: "'s \<Rightarrow> 'time"
-   init :: "'s \<Rightarrow> 's"
+   init :: "'s \<Rightarrow> 'reg \<Rightarrow> 's"
    stop_timer :: "'s \<Rightarrow> 's"
-   set_timeout :: "'s \<Rightarrow> 'timeout \<Rightarrow> bool \<Rightarrow> 's"
-   is_disabled :: "'s \<Rightarrow> bool"
+   set_timeout :: "'s \<Rightarrow> 'timeout \<Rightarrow> 'timer_mode \<Rightarrow> 's"
+   (* This is because the concrete get_time can trigger an overflow 
+      and we want to avoid this
+    *)
+   stateInv :: "'s \<Rightarrow> bool"
 
-
-record driver_state =
-  is_disabled :: "bool"
-(* difference with the original state *)
-  brightness :: nat
-  (* nleds :: nat *)
-
-(* what is the point of having bool^8 instead of 8 word? *)
-type_synonym device_colour = "8 word"
-
-term unat
-term uint
-find_theorems uint
-term word_of_int
-term Abs_word
-term word_of_nat
-find_consts nat "_ word"
-find_consts nat int
-
-
-fun serialise_channel :: "nat \<Rightarrow> 8 word \<Rightarrow> device_colour" where
-  "serialise_channel br r = 
-     word_of_int (int ((br * unat r) div 256))"
-
-
-record abstr_state =
-  driverState :: driver_state
-  deviceState :: "device_colour triple list"
-  
-
-definition abs_dataInv :: "abstr_state \<Rightarrow> bool"
-  where "abs_dataInv s = 
-      (length (leds (driverState s)) = length (deviceState s))" 
-
-(* brightness is a 8 word *)
-definition abs_driver :: "(abstr_state, nat, nat, 8 word, rgb) driver"
-  where
-  "abs_driver = 
-  \<lparr> 
-  
-   dataInv = (\<lambda> s. (length (leds (driverState s)) = length (deviceState s))
-   \<and> brightness (driverState s) \<le> (256 :: nat)
-           ),
-   brightnessInv = (\<lambda> b. True),
-   indexInv = (\<lambda> s i. i < length (leds (driverState s))),
-   get_nleds = (\<lambda> s. length (leds (driverState s))),
-   setB = (\<lambda>s b . s\<lparr>driverState := (driverState s)
-  \<comment> \<open>this definition is strange... \<close>
-   \<lparr>brightness := if b = 0 then 0 else unat b + 1\<rparr> \<rparr>) ,
-   setL = (\<lambda>s i c. s\<lparr>driverState := (driverState s)
-               \<lparr>leds := (leds (driverState s))[i := c]\<rparr> \<rparr>),
-   commit = (\<lambda> s . s\<lparr> deviceState := 
-                map (\<lambda> (w1, w2, w3) .
-                      (serialise_channel (brightness (driverState s)) w1,
-                       serialise_channel (brightness (driverState s)) w2,
-                       serialise_channel (brightness (driverState s)) w3)
-                      )
-                (leds (driverState s)) \<rparr>)
-\<rparr>"
-(*    
-*)
-locale driver_invariants =
-  fixes dr :: "('s, 'i, 'n, 'b, 'c) driver"
-  assumes
-    setBInv : "dataInv dr s \<Longrightarrow> brightnessInv dr b \<Longrightarrow>
-               dataInv dr (setB dr s b)"
-  assumes
-    setLInv : "dataInv dr s \<Longrightarrow> indexInv dr s i
-                   \<Longrightarrow> dataInv dr (setL dr s i c)"
-  assumes commitInv : 
-      "dataInv dr s \<Longrightarrow> dataInv dr (commit dr s)"
-
-interpretation abstr_implementation:
-  driver_invariants abs_driver
-  apply unfold_locales
-  apply ( simp add:abs_driver_def)
-
-record ('s1, 'i1, 'n1, 'b1, 'c1, 's2, 'i2, 'n2, 'b2, 'c2) 
+record ('s1, 'r1, 't1, 'to1, 'tm1, 
+        's2, 'r2, 't2, 'to2, 'tm2) 
   driver_morphism_rec =
   mor_state :: "'s1 \<Rightarrow> 's2" ("\<alpha>\<index>")
-  mor_index :: "'i1 \<Rightarrow> 'i2" ("\<alpha>index\<index>")
-  mor_brightness :: "'b1 \<Rightarrow> 'b2" (* abstract brightness *) ("\<alpha>brightness\<index>")
-  mor_length :: "'n1  \<Rightarrow> 'n2" ("\<alpha>length\<index>")
-  mor_colour :: "'c1 \<Rightarrow> 'c2" ("\<alpha>colour\<index>")
-
-type_synonym ('s, 'i, 'n, 'b, 'c) driver_abstr = 
-   "('s, 'i, 'n, 'b, 'c, 
-     abstr_state, nat, nat, 8 word, rgb) driver_morphism_rec"
-
-(*
-  fixes \<alpha> :: "'s1 \<Rightarrow> 's2"
-
-fixes \<alpha>index :: "'i1 \<Rightarrow> 'i2"
-fixes \<alpha>brightness :: "'b1 \<Rightarrow> 'b2" (* abstract brightness *)
-fixes \<alpha>length :: "'n1  \<Rightarrow> 'n2"
-fixes \<alpha>colour :: "'c1 \<Rightarrow> 'c2"*)
-
-(*
-locale driver_morphism =
-fixes \<alpha> :: "'s1 \<Rightarrow> 's2"
-fixes \<alpha>index :: "'i1 \<Rightarrow> 'i2"
-fixes \<alpha>brightness :: "'b1 \<Rightarrow> 'b2" (* abstract brightness *)
-fixes \<alpha>length :: "'n1  \<Rightarrow> 'n2"
-fixes \<alpha>colour :: "'c1 \<Rightarrow> 'c2"
-*)
+  mor_reg :: "'r1 \<Rightarrow> 'r2" ("\<alpha>reg\<index>")
+  mor_time :: "'t1 \<Rightarrow> 't2" ("\<alpha>time\<index>")
+  mor_timeout :: "'to1 \<Rightarrow> 'to2" ("\<alpha>timeout\<index>")
+  mor_timer_mode :: "'tm1  \<Rightarrow> 'tm2" ("\<alpha>timermode\<index>")
 
 locale driver_morphism_laws =  
 
 
-  fixes dr1 ::  "('s1, 'i1, 'n1, 'b1, 'c1) driver"
-  fixes dr2 :: "('s2, 'i2, 'n2, 'b2, 'c2) driver" 
- fixes mor :: "('s1, 'i1, 'n1, 'b1, 'c1, 's2, 'i2, 'n2, 'b2, 'c2) 
-   driver_morphism_rec"   (structure) 
+  fixes dr1 ::  "('s1, 'r1, 't1, 'to1, 'tm1) driver"
+  fixes dr2 :: "('s2, 'r2, 't2, 'to2, 'tm2) driver" 
+  fixes mor :: "('s1, 'r1, 't1, 'to1, 'tm1, 
+                 's2, 'r2, 't2, 'to2, 'tm2) driver_morphism_rec"   (structure) 
+  assumes \<alpha>get_time : "stateInv dr1 s \<Longrightarrow> get_time dr2 (\<alpha> s) = \<alpha>time (get_time dr1 s)"
+  assumes \<alpha>init : "init dr2 (\<alpha> s) (\<alpha>reg r) = \<alpha> (init dr1 s r)"
+  assumes \<alpha>stop_timer : "stop_timer dr2 (\<alpha> s) = \<alpha> (stop_timer dr1 s)"
+  assumes \<alpha>set_timeout : "   set_timeout dr2 (\<alpha> s) (\<alpha>timeout to) (\<alpha>timermode tm) = \<alpha> (set_timeout dr1 s to tm)"
 
-  
-(* assumes driver_morphism: "driver_morphism \<alpha> \<alpha>index \<alpha>brightness \<alpha>length \<alpha>colour" *)
+(* abstract driver *)
 
-assumes \<alpha>Inv : "dataInv dr1 s \<Longrightarrow> dataInv dr2 (\<alpha> s)"
+definition "ns_in_us = (1000 :: nat)"
 
-assumes \<alpha>indexInv : "dataInv dr1 s \<Longrightarrow> indexInv dr1 s i 
-               \<Longrightarrow> indexInv dr2 (\<alpha> s) (\<alpha>index i)"
+datatype timer_mode = Periodic | NotPeriodic
 
-assumes \<alpha>get_nleds : "dataInv dr1 s \<Longrightarrow> get_nleds dr2 (\<alpha> s) = \<alpha>length (get_nleds dr1 s)"
-assumes \<alpha>setB : "dataInv dr1 s \<Longrightarrow> brightnessInv dr1 b \<Longrightarrow>
-   setB dr2 (\<alpha> s) (\<alpha>brightness b) = \<alpha> (setB dr1 s b)"
-assumes \<alpha>setL : "dataInv dr1 s \<Longrightarrow> indexInv dr1 s i \<Longrightarrow>
-   setL dr2 (\<alpha> s) (\<alpha>index i) (\<alpha>colour c) = 
-       \<alpha> (setL dr1 s i c)"
-assumes \<alpha>commit : "dataInv dr1 s \<Longrightarrow>
-   commit dr2 (\<alpha> s) = \<alpha> (commit dr1 s)"
+datatype timestamp_timebase =
+  TIMESTAMP_TIMEBASE_SYSTEM
+  | TIMESTAMP_TIMEBASE_1_US
+  | TIMESTAMP_TIMEBASE_10_US
+  | TIMESTAMP_TIMEBASE_100_US
+  | TIMESTAMP_TIMEBASE_1_MS
+
+datatype timeout_timebase =
+   TIMEOUT_TIMEBASE_1_US
+ | TIMEOUT_TIMEBASE_10_US
+ | TIMEOUT_TIMEBASE_100_US
+ | TIMEOUT_TIMEBASE_1_MS
 
 
+record driver_state =
+  disable :: bool
+
+record device_state =
+  timer_a_mode :: timer_mode
+  timer_a_en :: bool
+  timer_a :: nat
+  timer_a_input_clk :: timeout_timebase
+  timer_e_input_clk :: timestamp_timebase
+  timer_e_low_hi :: nat
+
+
+record abstr_state =
+  driverState :: driver_state
+  deviceState :: device_state
+
+definition abs_driver :: "(abstr_state, device_state, nat, nat, timer_mode) driver"
+  where
+  "abs_driver = 
+\<lparr> get_time = (\<lambda> s. (timer_e_low_hi (deviceState s))  * (ns_in_us :: nat)),
+
+ init = (\<lambda> s r. s \<lparr> deviceState := r \<lparr>
+        timer_a_en := True
+      , timer_e_low_hi := 0
+      , timer_a_input_clk := TIMEOUT_TIMEBASE_1_MS
+      , timer_e_input_clk := TIMESTAMP_TIMEBASE_1_US
+ \<rparr> \<rparr>),
+
+ stop_timer = (\<lambda> s. \<lparr> 
+     driverState = \<lparr> disable = True \<rparr>,
+     deviceState = (deviceState s) \<lparr> timer_a_en := False \<rparr>
+     \<rparr>
+  ),
+
+set_timeout = (\<lambda> s timeout periodic. 
+  let deviceState' = (deviceState s) \<lparr>
+      timer_a := timeout,
+      timer_a_mode := periodic,
+      timer_a_en := 
+         if disable (driverState s) then
+           True
+         else
+           timer_a_en (deviceState s)
+      \<rparr>
+    in
+       \<lparr> driverState = \<lparr> disable = False \<rparr>,
+        deviceState = deviceState' \<rparr>
+   )
+   , stateInv = (\<lambda>s. True)
+
+\<rparr>
+"
+
+type_synonym ('s, 'r, 'time, 'timeout, 'timer_mode) driver_abstr = 
+   "('s, 'r, 'time, 'timeout, 'timer_mode, 
+     abstr_state, device_state, nat, nat, timer_mode) driver_morphism_rec"
 
 locale is_refinement = 
   driver_morphism_laws _ abs_driver mor
-  for mor :: "('s, 'i, 'n, 'b, 'c) driver_abstr"
-
-(*
-
-(* don't we want a kind of surjectivity as well? 
-Otherwise, I can just define a driver implementation whose invariant is 
-always wrong. Then, it will be a valid refinement... 
-
-This category is no longer locally presentable, but still accessible.
-*)
-locale driver_mor_epi =
-  driver_morphism dr1 dr2 \<alpha> \<alpha>index \<alpha>brightness \<alpha>length \<alpha>colour
-  for dr1 ::  "('s1, 'i1, 'n1, 'b1, 'c1) driver"
-   and dr2 ::  "('s2, 'i2, 'n2, 'b2, 'c2) driver"
-   and  \<alpha> \<alpha>index \<alpha>brightness \<alpha>length \<alpha>colour +
- fixes \<alpha>_section :: "'s2 \<Rightarrow> 's1"
- fixes \<alpha>index_section :: "'i2 \<Rightarrow> 'i1"
- fixes \<alpha>brightness_section :: "'b2 \<Rightarrow> 'b1" (* abstract brightness *)
-(* fixes \<alpha>length_section :: "'n2  \<Rightarrow> 'n1" 
-if dr2 = abs_driver, then this can be deduced.
-*)
- fixes \<alpha>colour_section :: "'c2 \<Rightarrow> 'c1"
-
-assumes \<alpha>_sectionInv :  "dataInv dr2 s \<Longrightarrow> dataInv dr1 (\<alpha>_section s)"
-assumes \<alpha>index_sectionInv : "dataInv dr2 s \<Longrightarrow> indexInv dr2 s i \<Longrightarrow>
-         indexInv dr1 (\<alpha>_section s) (\<alpha>index_section i)"
-
-assumes \<alpha>_section_eq :  "dataInv dr2 s \<Longrightarrow> \<alpha> ( \<alpha>_section s) = s"
-assumes \<alpha>index_section_eq : "dataInv dr2 s \<Longrightarrow> indexInv dr2 s i \<Longrightarrow>
-   \<alpha>index (\<alpha>index_section i) = i " 
-assumes \<alpha>brightness_section : "\<alpha>brightness \<circ> \<alpha>brightness_section = id"
-(*
-assumes \<alpha>length_section : "\<alpha>length \<circ> \<alpha>length_section = id"
-*)
-assumes \<alpha>colour_section : "\<alpha>colour \<circ> \<alpha>colour_section = id"
-
-(* Note: I should define invariants for brightness (< 255) and color *)
-definition is_refinement_epi :: 
-  "('s, 'i, 'n, 'b, 'c) driver \<Rightarrow>
-    ('s \<Rightarrow> _) \<Rightarrow> ('i \<Rightarrow> _) \<Rightarrow> ('b \<Rightarrow> _) \<Rightarrow> ('n \<Rightarrow> _) \<Rightarrow> ('c \<Rightarrow> _) \<Rightarrow>
-   _ \<Rightarrow> _ \<Rightarrow> _ \<Rightarrow> _ \<Rightarrow>
- bool"
-  where "is_refinement_epi dr 
-  \<alpha> \<alpha>index \<alpha>brightness \<alpha>length \<alpha>colour
-  \<alpha>_section \<alpha>index_section \<alpha>brightness_section \<alpha>colour_section
- = 
-(driver_mor_epi dr abs_driver \<alpha> \<alpha>index \<alpha>brightness \<alpha>length \<alpha>colour
-  \<alpha>_section \<alpha>index_section \<alpha>brightness_section \<alpha>colour_section)"
-
-*)
-
-
-subsection \<open>Concrete Refinement\<close>
-
-subsubsection \<open>Helpers\<close>
-
-fun extract_Error :: "('a, 'a) Error \<Rightarrow> 'a" where
-  "extract_Error (Ok a) = a"
-| "extract_Error (Err a) = a"
-
-fun curry_T1 :: "(('a, 'b) T1 \<Rightarrow> 'c) \<Rightarrow> ('a \<Rightarrow> 'b \<Rightarrow> 'c)" where
-  "curry_T1 f a b = f (\<lparr> T1.p1\<^sub>f = a, p2\<^sub>f = b \<rparr>)"
-
-fun uncurry_T1 :: "('a \<Rightarrow> 'b \<Rightarrow> 'c) \<Rightarrow> (('a, 'b) T1 \<Rightarrow> 'c)" where
-  "uncurry_T1 f (\<lparr> T1.p1\<^sub>f = a, p2\<^sub>f = b \<rparr>) = f a b"
-
-fun curry_T0 :: "(('a, 'b, 'c, 'd, 'e) T0 \<Rightarrow> 'z) \<Rightarrow> ('a \<Rightarrow> 'b \<Rightarrow> 'c \<Rightarrow> 'd \<Rightarrow> 'e \<Rightarrow> 'z)" where
-  "curry_T0 f a b c d e = f (\<lparr> T0.p1\<^sub>f = a, p2\<^sub>f = b, p3\<^sub>f = c, p4\<^sub>f = d, p5\<^sub>f = e \<rparr>)"
-
-fun uncurry_T0 :: "('a \<Rightarrow> 'b \<Rightarrow> 'c \<Rightarrow> 'd \<Rightarrow> 'e \<Rightarrow> 'z) \<Rightarrow> (('a, 'b, 'c, 'd, 'e) T0 \<Rightarrow> 'z)" where
-  "uncurry_T0 f (\<lparr> T0.p1\<^sub>f = a, p2\<^sub>f = b, p3\<^sub>f = c, p4\<^sub>f = d, p5\<^sub>f = e \<rparr>) = f a b c d e"
-
-
-subsubsection \<open>Concrete driver\<close>
-
-fun ws_set_led' :: "Wsp\<^sub>T \<Rightarrow> 32 word \<Rightarrow> (8 word \<times> 8 word \<times> 8 word) \<Rightarrow> Wsp\<^sub>T" where
-  "ws_set_led' s i (r,g,b) = curry_T0 (ws_set_led) s i r g b"
-
-
-
-definition wsp_length_correctness_condition :: "Wsp\<^sub>T \<Rightarrow> bool" where
-  "wsp_length_correctness_condition (r :: Wsp\<^sub>T) \<equiv>
-    length (led_data\<^sub>f r) = length (led_state\<^sub>f r)
-    \<and> length (led_state\<^sub>f r) < 0xFFFFFFFF"
-
-
-definition concr_driver :: "(Wsp\<^sub>T, 32 word, nat, 32 word, 8 word triple) driver"
-  where
-  "concr_driver = 
-  \<lparr> 
-  
-   dataInv = wsp_length_correctness_condition,
-   brightnessInv = (\<lambda> b. unat b < 256),
-   indexInv = (\<lambda> s i. unat i < length (led_data\<^sub>f s)),
-\<comment> \<open>difference with the original implementation: not 8\<close>
-   get_nleds = (\<lambda> s.  ( length (led_data\<^sub>f s))),
-   setB = curry_T1 (extract_Error \<circ> ws_set_brightness) ,
-   setL = ws_set_led' ,
-   commit = ws_commit 
-\<rparr>"
-
-locale concr_is_refinement = 
-  is_refinement concr_driver mor
-  for mor :: "(Wsp\<^sub>T, 32 word, nat, 32 word, 8 word triple) driver_abstr"
-
-
-
-
-subsection \<open>Abstraction Definitions\<close>
-
-
-type_synonym LEDArray = "Rgb\<^sub>T list"
-type_synonym led = "8 word triple"
-type_synonym LEDData = "RgbX\<^sub>T list"
-
-definition extract_led_arr_val :: "LEDArray \<Rightarrow> led list" where
-  "extract_led_arr_val xs = map (\<lambda>grb. (g\<^sub>f grb, r\<^sub>f grb, b\<^sub>f grb)) xs"
-
-lemma extract_led_arr_val_length[simp]:
-  shows "length (extract_led_arr_val xs) = length xs"
-  by (simp add: extract_led_arr_val_def)
-
-lemma extract_led_arr_val_nth:
-  assumes "i < length xs"
-  shows "extract_led_arr_val xs ! i = (g\<^sub>f (xs ! i), r\<^sub>f (xs ! i), b\<^sub>f (xs ! i))"
-  using assms
-  by (simp add: extract_led_arr_val_def)
-
-(* inverse of expand_channel *)
-definition split_led_encoding :: "32 word \<Rightarrow> 8 word" where
-  "split_led_encoding w = 
-    (let encode = (\<lambda>w. (if w = (0x88 :: 8 word) then (0 :: 8 word)
-                        else if w = (0x8c :: 8 word) then 1
-                        else if w = (0xc8 :: 8 word) then 2
-                        else if w = (0xcc :: 8 word) then 3
-                        else undefined))
-     in    (encode (ucast ((w >> 24) && 0xFF)) << 6)
-       ||  (encode (ucast ((w >> 16) && 0xFF)) << 4)
-       ||  (encode (ucast ((w >> 8) && 0xFF)) << 2)
-       ||  (encode (ucast (w && 0xFF)))
-)"
-lemma saveme : 
-    "split_led_encoding (expand_channel x) 
-   =  SCAST(32 \<rightarrow> 8) x
-    "
-  sorry
-
-
- definition extract_led_data_val :: "LEDData \<Rightarrow> device_colour triple list" where
-  "extract_led_data_val as = map (\<lambda>a. (split_led_encoding (gx\<^sub>f a), split_led_encoding (rx\<^sub>f a), split_led_encoding (bx\<^sub>f a))) as"
- 
- lemma extract_led_data_val_length[simp]:
-  "length (extract_led_data_val xs) = length xs"
-  by (simp add: extract_led_data_val_def) 
-
- lemma extract_led_data_val_nth:
-  assumes "i < length xs"
-  shows "extract_led_data_val xs ! i = (split_led_encoding (gx\<^sub>f (xs ! i)), split_led_encoding (rx\<^sub>f (xs ! i)), split_led_encoding (bx\<^sub>f (xs ! i)))"
-  using assms
-  by (simp add: extract_led_data_val_def) 
-
-
-subsection \<open>Concrete Abstraction Functions\<close>
-
-definition \<alpha>Wsp\<^sub>T :: "Wsp\<^sub>T \<Rightarrow> abstr_state" where
-  "\<alpha>Wsp\<^sub>T r = 
-   \<lparr> driverState = \<lparr> leds = extract_led_arr_val (led_state\<^sub>f r),
-     brightness = ucast (brightness\<^sub>f r) \<rparr>, 
-     deviceState = extract_led_data_val (led_data\<^sub>f r) \<rparr>"
-
-definition abstraction :: "(Wsp\<^sub>T, 32 word, nat, 32 word, 8 word triple) driver_abstr"
-  where "abstraction = 
-  \<lparr>
-   mor_state = \<alpha>Wsp\<^sub>T,
-   mor_index = unat,
-   mor_brightness = ucast, 
-   mor_length = id,
-   mor_colour = id 
-  \<rparr>"
-
-(*
-definition serialise_led :: "nat \<Rightarrow> led \<Rightarrow> device_colour triple" where
-  "serialise_led br led = (serialise_channel br (\<alpha>g led), serialise_channel br (\<alpha>r led), serialise_channel br (\<alpha>b led))"
-
-
-definition leds_to_device_state :: "nat \<Rightarrow> led list \<Rightarrow> device_state" where
-  "leds_to_device_state br led_list \<equiv> map (serialise_led br) led_list"
-*)
-
-lemmas driver_defs = concr_driver_def abs_driver_def abstraction_def
-lemmas simp_defs = driver_defs
-   wsp_length_correctness_condition_def \<alpha>Wsp\<^sub>T_def
-
-lemmas cogent_defs = 
-Let_def  take\<^sub>c\<^sub>o\<^sub>g\<^sub>e\<^sub>n\<^sub>t_def Let\<^sub>d\<^sub>s_def T1.defs 
-
-lemma map2_fst_trivial:
-  assumes "length xs = length ys"
-  shows "fst (array_map2 (\<lambda>x y. (f x, g x y)) xs ys) = map f xs"
-  using assms
-  by (induct rule: list_induct2) (clarsimp split: prod.splits)+
-
-lemma map2_snd_trivial:
-  assumes "length xs = length ys"
-  shows "snd (array_map2 (\<lambda>x y. (f x, g x y)) xs ys) = map2 g xs ys"
-  using assms
-  by (induct rule: list_induct2) (clarsimp split: prod.splits)+
-
-lemma map2_snd_trivial':
-  assumes "length xs = length ys"
-  shows "snd (array_map2 (\<lambda>x y. (f x, g x)) xs ys) = map g xs"
-  using assms
-  by (induct rule: list_induct2) (clarsimp split: prod.splits)+
-
-
-(*
-definition unzip :: "('a \<times> 'b) list \<Rightarrow> 'a list \<times> 'b list"
-  where "unzip l = (map fst l, map snd l)"
-lemma array_map2_spec :
-  assumes "length l1 = length l2"
-  shows
-  "array_map2 f l1 l2 =
-   unzip ( map2 f l1 l2)"
-  using assms
-  apply (induct rule: list_induct2) 
-   apply (simp add:unzip_def)
-  apply (simp add:unzip_def)  
-  using case_prod_beta by blast
-
-*)
-
-lemma elim_rgb : "ds \<lparr> gx\<^sub>f := g,
-                    rx\<^sub>f := r,
-                    bx\<^sub>f := b\<rparr> = 
-                  \<lparr> gx\<^sub>f = g,
-                    rx\<^sub>f = r,
-                    bx\<^sub>f = b\<rparr>
-"
-  by simp
-
-lemma chiant : "unat (n ) < 2^LENGTH('a :: len) \<Longrightarrow>
- n = ucast (of_nat (unat n) :: 'a word)"
-  apply(simp add:ucast_def unat_def)
-  apply(simp add: word_ubin.eq_norm word_of_int bintrunc_mod2p )
-  done
-
-lemma chiant2 : "unat (n ) < 2^LENGTH('a :: len) \<Longrightarrow>
-\<exists> p.  n = ucast (p :: 'a word)"
-  apply (drule chiant)
-  by blast
-
-
-lemma commit_refinement':
-  assumes "wsp_length_correctness_condition s"
-  shows "\<alpha>Wsp\<^sub>T (ws_commit s) = commit abs_driver (\<alpha>Wsp\<^sub>T s)"
-(*
- \<lparr> driverState = driverState (\<alpha>Wsp\<^sub>T s),
-   deviceState = leds_to_device_state (brightness (driverState (\<alpha>Wsp\<^sub>T s))) (leds (driverState (\<alpha>Wsp\<^sub>T s))) \<rparr>"
-*)
-  using assms
-  apply (simp add:simp_defs)
-  
-  
-  
-  apply(simp add:ws_commit_def cogent_defs expand_def)
-  apply(intro conjI)+
-  apply(simp add:map2_fst_trivial) 
-(*   apply(simp add:array_map2_spec unzip_def) *)
-  
-  apply(simp add:elim_rgb map2_snd_trivial')
-  
-  (*apply (simp add:array_map2_spec unzip_def) *)
-  apply(simp add:extract_led_arr_val_def)
-  apply (simp add:extract_led_data_val_def)
-  term "(checked_div (brightness\<^sub>f s * UCAST(8 \<rightarrow> 32) (g\<^sub>f x)) 0x100)"
-  by(simp add:saveme)
-
-interpretation concr_implementation:
-  concr_is_refinement abstraction
-  apply unfold_locales
-  (* preservation of state invariant *)
-       apply (simp add:simp_defs)
-      apply (simp add:simp_defs)
-     apply (simp add:simp_defs)
-(* brightness *)
-   apply(simp add:simp_defs)  
-apply (
-      simp add: \<alpha>Wsp\<^sub>T_def ws_set_brightness_def take\<^sub>c\<^sub>o\<^sub>g\<^sub>e\<^sub>n\<^sub>t_def unat_eq_zero word_less_nat_alt
-      unat_plus_if' wsp_length_correctness_condition_def)
-    apply(intro impI conjI)+
-  
-     apply(simp add:ucast_def)
-     apply(simp only:Word.word.uint_inject[of _ 0, symmetric])
-     apply(simp add: unat_def word_ubin.eq_norm word_of_int bintrunc_mod2p )
-    apply(simp add:ucast_def)
-    apply(simp only:Word.word.uint_inject[ symmetric])
-    apply(simp add: unat_def word_ubin.eq_norm word_of_int bintrunc_mod2p )
-
-
-  find_theorems uint name:inj
-  thm word_ubin.eq_norm word_of_int
-  find_theorems word_of_int
-  find_theorems uint ucast
-  
-  find_theorems uint
-  find_theorems is_up
-  find_theorems ucast uint
-  find_theorems ucast
-  term of_bl
-  
-     apply (word_bitwise)
-  
-  find_theorems ucast 
-(* set_led *)
-  apply(simp add:simp_defs)  
- apply (force split: prod.splits simp add: 
-
- T1.defs ws_set_led_def \<alpha>Wsp\<^sub>T_def take\<^sub>c\<^sub>o\<^sub>g\<^sub>e\<^sub>n\<^sub>t_def
-      Let_def Rgb.defs list_eq_iff_nth_eq nth_list_update extract_led_arr_val_def
-      wsp_length_correctness_condition_def)
-
-(* commit *)
-  by(simp add: driver_defs commit_refinement')
+  for mor :: "('s, 'r, 'time, 'timeout, 'timer_mode) driver_abstr"
   
 end
