timer/Refinement.thy
@@ -1,0 +1,169 @@
+theory Refinement
+  imports Main "HOL-Word.Word" "Word_Lib.Word_Lib" "TimerSpec"
+(* should be dargentfull*)
+ "build_ignore_volatile_wo_u23/Ignore_volatile_wo_u23_dargentfull_Shallow_Desugar"
+begin
+
+fun curry_T0 :: "(('a, 'b, 'c) T0 \<Rightarrow> 'z) \<Rightarrow> ('a \<Rightarrow> 'b \<Rightarrow> 'c \<Rightarrow> 'z)" where
+  "curry_T0 f a b c = f (\<lparr> T0.p1\<^sub>f = a, p2\<^sub>f = b, p3\<^sub>f = c \<rparr>)"
+
+fun curry_T3 :: "(('a, 'b) T1 \<Rightarrow> 'c) \<Rightarrow> ('a \<Rightarrow> 'b \<Rightarrow> 'c)" where
+  "curry_T3 f a b = f (\<lparr> T1.p1\<^sub>f = a, p2\<^sub>f = b \<rparr>)"
+
+axiomatization
+  where cast82_def:"cast82 x = x && 0b11"
+   and  cast83_def:"cast83 x = x && 0b111"
+
+
+
+type_synonym concr_device_state = "(bool, bool, 8 word, 8 word, 32 word, 32 word, 32 word) Meson_timer_reg"
+type_synonym concr_state = "(concr_device_state, bool) Meson_timer"
+
+definition concr_driver :: "(concr_state, VAddr, 64 word, 16 word, bool) driver"
+  where
+  "concr_driver = 
+\<lparr> 
+  get_time = meson_get_time,
+  init = curry_T3 meson_init,
+  stop_timer = meson_stop_timer,
+  set_timeout = curry_T0 meson_set_timeout,
+\<comment> \<open>we are going to multiply it by 1000 (\<approx> 1024 = 2^10) \<close>
+  stateInv = (\<lambda>s.  timer_e_hi\<^sub>f (regs\<^sub>f s) < 2^(32-10))
+\<rparr>
+"
+
+locale concr_is_refinement = 
+  is_refinement concr_driver mor
+  for mor :: "(concr_state, VAddr, 64 word, 16 word, bool) driver_abstr"
+
+definition \<alpha>timeout_timebase :: "nat \<Rightarrow> timeout_timebase"
+  where 
+  "\<alpha>timeout_timebase n = 
+   (if n = 0 then TIMEOUT_TIMEBASE_1_US   else
+    if n = 1 then TIMEOUT_TIMEBASE_10_US  else
+    if n = 2 then TIMEOUT_TIMEBASE_100_US else
+    if n = 3 then TIMEOUT_TIMEBASE_1_MS   else
+    undefined)
+   "
+   
+definition \<alpha>timestamp_timebase :: "nat \<Rightarrow> timestamp_timebase"
+  where 
+  "\<alpha>timestamp_timebase n = 
+   (if n = 0 then TIMESTAMP_TIMEBASE_SYSTEM   else
+    if n = 1 then TIMESTAMP_TIMEBASE_1_US  else
+    if n = 2 then TIMESTAMP_TIMEBASE_10_US else
+    if n = 3 then TIMESTAMP_TIMEBASE_100_US   else
+    if n = 4 then TIMESTAMP_TIMEBASE_100_US   else
+    TIMESTAMP_TIMEBASE_1_MS)
+   "
+
+definition \<alpha>_timer_mode :: "bool \<Rightarrow> timer_mode"
+  where "\<alpha>_timer_mode b = (if b then Periodic else NotPeriodic)"
+term word_cat
+definition \<alpha>_reg :: "concr_device_state \<Rightarrow> device_state" where
+"\<alpha>_reg ds = 
+    \<lparr> timer_a_mode = \<alpha>_timer_mode (timer_a_mode\<^sub>f ds) ,
+     timer_a_en = timer_a_en\<^sub>f ds,
+timer_a = unat (timer_a\<^sub>f ds),
+timer_a_input_clk = \<alpha>timeout_timebase (unat (timer_a_input_clk\<^sub>f ds)),
+timer_e_input_clk = \<alpha>timestamp_timebase (unat (timer_e_input_clk\<^sub>f ds)),
+timer_e_low_hi = unat (word_cat (timer_e_hi\<^sub>f ds) (timer_e\<^sub>f ds) :: 64 word)
+
+ \<rparr> "
+
+definition \<alpha>_state :: "concr_state \<Rightarrow> abstr_state" where
+"\<alpha>_state s = 
+  \<lparr> 
+    driverState = \<lparr> disable = disable\<^sub>f s \<rparr>,
+    deviceState = \<alpha>_reg (regs\<^sub>f s)
+  \<rparr>"
+
+definition abstraction :: "(concr_state, VAddr, 64 word, 16 word, bool) driver_abstr"
+  where "abstraction = 
+  \<lparr>
+   mor_state = \<alpha>_state,
+   mor_reg = \<alpha>_reg o config_get_regs,
+   mor_time = unat, 
+   mor_timeout = unat,
+   mor_timer_mode = \<alpha>_timer_mode 
+  \<rparr>"
+
+lemmas driver_defs = concr_driver_def abs_driver_def abstraction_def
+lemmas simp_defs = driver_defs \<alpha>_state_def \<alpha>_reg_def \<alpha>timeout_timebase_def
+ \<alpha>timestamp_timebase_def
+
+
+thm unat_def uint_up_ucast is_up
+
+lemma unat_ucast_up : 
+ " LENGTH('a :: len0) \<le> LENGTH('b ::len0) \<Longrightarrow> 
+unat (UCAST('a \<rightarrow> 'b) w) = unat w"
+  by (simp add: unat_def uint_up_ucast is_up)
+
+
+lemma helper1 : "
+((UCAST(32 \<rightarrow> 64) x << 32) || UCAST(32 \<rightarrow> 64) y)
+= word_cat x y"
+  by word_bitwise
+
+lemma helper2 : "
+(h :: int) < 4194304 \<Longrightarrow> l < 2^32 \<Longrightarrow> 536870912000 * h + 125 * l < 2305843009213693952
+"  
+  
+  apply(rule less_le_trans)
+   apply(rule add_strict_mono)
+    apply(erule mult_strict_left_mono)
+    apply simp
+   apply(erule mult_strict_left_mono)
+   apply simp
+  apply simp
+  done
+
+
+interpretation concr_implementation:
+  concr_is_refinement abstraction
+  apply unfold_locales
+     apply (simp add:simp_defs meson_get_time_def ns_in_us_def)
+
+     apply(case_tac s, rename_tac regs disable, case_tac regs)
+     apply clarsimp
+     apply(simp add:helper1)
+     apply(simp add:unat_def)
+     apply (subst uint_mult_lem[THEN HOL.iffD1])
+      apply simp
+      apply(simp add:word_cat_def )
+      apply(subst word_ubin.eq_norm)
+ 
+      apply simp
+      apply(simp add:bintr_cat)
+      apply(subst word_ubin.norm_norm(2)[THEN fun_cong, simplified comp_def, of "_ :: 32 word", simplified])
+      apply(simp add:bin_cat_num)
+      apply(subst word_ubin.norm_norm(2)[THEN fun_cong, simplified comp_def, of "_ :: 32 word", simplified])
+      apply(simp add:word_less_alt)
+      apply(erule helper2)
+
+
+      apply(uint_arith, simp)
+     apply simp
+
+
+apply (simp add:simp_defs meson_init_def meson_get_time_def ns_in_us_def)
+     apply(case_tac s, rename_tac regs disable, case_tac regs)
+    apply(simp add: take\<^sub>c\<^sub>o\<^sub>g\<^sub>e\<^sub>n\<^sub>t_def cast82_def cast83_def)
+     (* hmm *)
+     apply clarsimp
+(* it should work because setting 
+the lower register should set the higher register
+*)
+  defer
+
+(* yeah! *)
+     apply (simp add:simp_defs meson_stop_timer_def  ns_in_us_def take\<^sub>c\<^sub>o\<^sub>g\<^sub>e\<^sub>n\<^sub>t_def)
+
+  
+    
+    apply(simp add:simp_defs  meson_set_timeout_def  take\<^sub>c\<^sub>o\<^sub>g\<^sub>e\<^sub>n\<^sub>t_def Let\<^sub>d\<^sub>s_def)
+    apply(simp add:unat_ucast_up)
+  sorry
+
+end
